examples/ghc/lib/CoreArity.v
@@ -1,0 +1,128 @@
+(* Default settings (from HsToCoq.Coq.Preamble) *)
+
+Generalizable All Variables.
+
+Unset Implicit Arguments.
+Set Maximal Implicit Insertion.
+Unset Strict Implicit.
+Unset Printing Implicit Defensive.
+
+Require Coq.Program.Tactics.
+Require Coq.Program.Wf.
+
+(* Converted imports: *)
+
+Require AxiomatizedTypes.
+Require BasicTypes.
+Require Core.
+Require CoreSubst.
+Require CoreUtils.
+Require DynFlags.
+Require GHC.Err.
+
+(* Converted type declarations: *)
+
+Inductive EtaInfo : Type
+  := | EtaVar : Core.Var -> EtaInfo
+  |  EtaCo : AxiomatizedTypes.Coercion -> EtaInfo.
+
+Definition CheapFun :=
+  (Core.CoreExpr -> option AxiomatizedTypes.Type_ -> bool)%type.
+
+Inductive ArityType : Type
+  := | ATop : list BasicTypes.OneShotInfo -> ArityType
+  |  ABot : BasicTypes.Arity -> ArityType.
+
+Inductive ArityEnv : Type
+  := | AE (ae_cheap_fn : CheapFun) (ae_ped_bot : bool) : ArityEnv.
+
+Instance Default__ArityEnv : GHC.Err.Default ArityEnv :=
+  GHC.Err.Build_Default _ (AE GHC.Err.default GHC.Err.default).
+
+Definition ae_cheap_fn (arg_0__ : ArityEnv) :=
+  let 'AE ae_cheap_fn _ := arg_0__ in
+  ae_cheap_fn.
+
+Definition ae_ped_bot (arg_0__ : ArityEnv) :=
+  let 'AE _ ae_ped_bot := arg_0__ in
+  ae_ped_bot.
+
+(* Converted value declarations: *)
+
+Axiom vanillaArityType : ArityType.
+
+Axiom typeArity : AxiomatizedTypes.Type_ -> list BasicTypes.OneShotInfo.
+
+Axiom subst_expr : CoreSubst.Subst -> Core.CoreExpr -> Core.CoreExpr.
+
+Axiom pushCoercion : AxiomatizedTypes.Coercion -> list EtaInfo -> list EtaInfo.
+
+Axiom mk_cheap_fn : DynFlags.DynFlags -> CoreUtils.CheapAppFun -> CheapFun.
+
+Axiom mkEtaWW : BasicTypes.Arity ->
+                Core.CoreExpr ->
+                Core.InScopeSet ->
+                AxiomatizedTypes.Type_ -> (Core.InScopeSet * list EtaInfo)%type.
+
+Axiom manifestArity : Core.CoreExpr -> BasicTypes.Arity.
+
+Axiom joinRhsArity : Core.CoreExpr -> BasicTypes.JoinArity.
+
+Axiom getBotArity : ArityType -> option BasicTypes.Arity.
+
+Axiom freshEtaId : nat ->
+                   Core.TCvSubst -> AxiomatizedTypes.Type_ -> (Core.TCvSubst * Core.Id)%type.
+
+Axiom floatIn : bool -> ArityType -> ArityType.
+
+Axiom findRhsArity : DynFlags.DynFlags ->
+                     Core.Id -> Core.CoreExpr -> BasicTypes.Arity -> (BasicTypes.Arity * bool)%type.
+
+Axiom exprEtaExpandArity : DynFlags.DynFlags ->
+                           Core.CoreExpr -> BasicTypes.Arity.
+
+Axiom exprBotStrictness_maybe : Core.CoreExpr ->
+                                option (BasicTypes.Arity * Core.StrictSig)%type.
+
+Axiom exprArity : Core.CoreExpr -> BasicTypes.Arity.
+
+Axiom etaInfoAppTy : AxiomatizedTypes.Type_ ->
+                     list EtaInfo -> AxiomatizedTypes.Type_.
+
+Axiom etaInfoApp : CoreSubst.Subst ->
+                   Core.CoreExpr -> list EtaInfo -> Core.CoreExpr.
+
+Axiom etaInfoAbs : list EtaInfo -> Core.CoreExpr -> Core.CoreExpr.
+
+Axiom etaExpandToJoinPointRule : BasicTypes.JoinArity ->
+                                 Core.CoreRule -> Core.CoreRule.
+
+Axiom etaExpandToJoinPoint : BasicTypes.JoinArity ->
+                             Core.CoreExpr -> (list Core.CoreBndr * Core.CoreExpr)%type.
+
+Axiom etaExpand : BasicTypes.Arity -> Core.CoreExpr -> Core.CoreExpr.
+
+Axiom etaBodyForJoinPoint : nat ->
+                            Core.CoreExpr -> (list Core.CoreBndr * Core.CoreExpr)%type.
+
+Axiom arityType : ArityEnv -> Core.CoreExpr -> ArityType.
+
+Axiom arityLam : Core.Id -> ArityType -> ArityType.
+
+Axiom arityApp : ArityType -> bool -> ArityType.
+
+Axiom andArityType : ArityType -> ArityType -> ArityType.
+
+(* Skipping all instances of class `Outputable.Outputable', including
+   `CoreArity.Outputable__ArityType' *)
+
+(* Skipping all instances of class `Outputable.Outputable', including
+   `CoreArity.Outputable__EtaInfo' *)
+
+(* External variables:
+     bool list nat op_zt__ option AxiomatizedTypes.Coercion AxiomatizedTypes.Type_
+     BasicTypes.Arity BasicTypes.JoinArity BasicTypes.OneShotInfo Core.CoreBndr
+     Core.CoreExpr Core.CoreRule Core.Id Core.InScopeSet Core.StrictSig Core.TCvSubst
+     Core.Var CoreSubst.Subst CoreUtils.CheapAppFun DynFlags.DynFlags
+     GHC.Err.Build_Default GHC.Err.Default GHC.Err.default
+*)
