examples/ghc/lib/TysWiredIn.v
@@ -1,0 +1,456 @@
+(* Default settings (from HsToCoq.Coq.Preamble) *)
+
+Generalizable All Variables.
+
+Unset Implicit Arguments.
+Set Maximal Implicit Insertion.
+Unset Strict Implicit.
+Unset Printing Implicit Defensive.
+
+Require Coq.Program.Tactics.
+Require Coq.Program.Wf.
+
+(* Converted imports: *)
+
+Require AxiomatizedTypes.
+Require BasicTypes.
+Require Core.
+Require FastString.
+Require GHC.Base.
+Require Module.
+Require Name.
+Require NameEnv.
+Require NameSet.
+Require OccName.
+Require PrelNames.
+Require Unique.
+
+(* No type declarations to convert. *)
+
+(* Converted value declarations: *)
+
+Axiom wordTyConName : Name.Name.
+
+Axiom wordTyCon : Core.TyCon.
+
+Axiom wordTy : AxiomatizedTypes.Type_.
+
+Axiom wordDataConName : Name.Name.
+
+Axiom wordDataCon : Core.DataCon.
+
+Axiom word8TyConName : Name.Name.
+
+Axiom word8TyCon : Core.TyCon.
+
+Axiom word8Ty : AxiomatizedTypes.Type_.
+
+Axiom word8DataConName : Name.Name.
+
+Axiom word8DataCon : Core.DataCon.
+
+Axiom wiredInTyCons : list Core.TyCon.
+
+Axiom vecRepDataConTyCon : Core.TyCon.
+
+Axiom vecRepDataConName : Name.Name.
+
+Axiom vecRepDataCon : Core.DataCon.
+
+Axiom vecElemTyConName : Name.Name.
+
+Axiom vecElemTyCon : Core.TyCon.
+
+Axiom vecElemDataCons : list Core.DataCon.
+
+Axiom vecElemDataConNames : list Name.Name.
+
+Axiom vecCountTyConName : Name.Name.
+
+Axiom vecCountTyCon : Core.TyCon.
+
+Axiom vecCountDataCons : list Core.DataCon.
+
+Axiom vecCountDataConNames : list Name.Name.
+
+Axiom unitTyConKey : Unique.Unique.
+
+Axiom unitTyCon : Core.TyCon.
+
+Axiom unitTy : AxiomatizedTypes.Type_.
+
+Axiom unitDataConId : Core.Id.
+
+Axiom unitDataCon : Core.DataCon.
+
+Axiom unicodeStarKindTyConName : Name.Name.
+
+Axiom unicodeStarKindTyCon : Core.TyCon.
+
+Axiom unboxedUnitTyCon : Core.TyCon.
+
+Axiom unboxedUnitDataCon : Core.DataCon.
+
+Axiom unboxedTupleSumKind : Core.TyCon ->
+                            list AxiomatizedTypes.Type_ -> AxiomatizedTypes.Kind.
+
+Axiom unboxedTupleKind : list AxiomatizedTypes.Type_ -> AxiomatizedTypes.Kind.
+
+Axiom unboxedSumKind : list AxiomatizedTypes.Type_ -> AxiomatizedTypes.Kind.
+
+Axiom typeSymbolKindConName : Name.Name.
+
+Axiom typeSymbolKindCon : Core.TyCon.
+
+Axiom typeSymbolKind : AxiomatizedTypes.Kind.
+
+Axiom typeNatKindConName : Name.Name.
+
+Axiom typeNatKindCon : Core.TyCon.
+
+Axiom typeNatKind : AxiomatizedTypes.Kind.
+
+Axiom tupleTyConName : BasicTypes.TupleSort -> BasicTypes.Arity -> Name.Name.
+
+Axiom tupleTyCon : BasicTypes.Boxity -> BasicTypes.Arity -> Core.TyCon.
+
+Axiom tupleRepDataConTyCon : Core.TyCon.
+
+Axiom tupleRepDataConName : Name.Name.
+
+Axiom tupleRepDataCon : Core.DataCon.
+
+Axiom tupleDataCon : BasicTypes.Boxity -> BasicTypes.Arity -> Core.DataCon.
+
+Axiom true_RDR : PrelNames.RdrName.
+
+Axiom trueDataConName : Name.Name.
+
+Axiom trueDataConId : Core.Id.
+
+Axiom trueDataCon : Core.DataCon.
+
+Axiom sumTyCon : BasicTypes.Arity -> Core.TyCon.
+
+Axiom sumRepDataConTyCon : Core.TyCon.
+
+Axiom sumRepDataConName : Name.Name.
+
+Axiom sumRepDataCon : Core.DataCon.
+
+Axiom sumDataCon : BasicTypes.ConTag -> BasicTypes.Arity -> Core.DataCon.
+
+Axiom stringTy : AxiomatizedTypes.Type_.
+
+Axiom starKindTyConName : Name.Name.
+
+Axiom starKindTyCon : Core.TyCon.
+
+Axiom runtimeRepTyConName : Name.Name.
+
+Axiom runtimeRepTyCon : Core.TyCon.
+
+Axiom runtimeRepTy : AxiomatizedTypes.Type_.
+
+Axiom runtimeRepSimpleDataConNames : list Name.Name.
+
+Axiom promotedTupleDataCon : BasicTypes.Boxity ->
+                             BasicTypes.Arity -> Core.TyCon.
+
+Axiom promotedTrueDataCon : Core.TyCon.
+
+Axiom promotedNothingDataCon : Core.TyCon.
+
+Axiom promotedNilDataCon : Core.TyCon.
+
+Axiom promotedLTDataCon : Core.TyCon.
+
+Axiom promotedJustDataCon : Core.TyCon.
+
+Axiom promotedGTDataCon : Core.TyCon.
+
+Axiom promotedFalseDataCon : Core.TyCon.
+
+Axiom promotedEQDataCon : Core.TyCon.
+
+Axiom promotedConsDataCon : Core.TyCon.
+
+Axiom pcTyCon : bool ->
+                Name.Name ->
+                option AxiomatizedTypes.CType ->
+                list Core.TyVar -> list Core.DataCon -> Core.TyCon.
+
+Axiom pcSpecialDataCon : Name.Name ->
+                         list AxiomatizedTypes.Type_ ->
+                         Core.TyCon -> Core.RuntimeRepInfo -> Core.DataCon.
+
+Axiom pcNonEnumTyCon : Name.Name ->
+                       option AxiomatizedTypes.CType ->
+                       list Core.TyVar -> list Core.DataCon -> Core.TyCon.
+
+Axiom pcDataConWithFixity' : bool ->
+                             Name.Name ->
+                             Unique.Unique ->
+                             Core.RuntimeRepInfo ->
+                             list Core.TyVar ->
+                             list Core.TyVar ->
+                             list Core.TyVar -> list AxiomatizedTypes.Type_ -> Core.TyCon -> Core.DataCon.
+
+Axiom pcDataConWithFixity : bool ->
+                            Name.Name ->
+                            list Core.TyVar ->
+                            list Core.TyVar ->
+                            list Core.TyVar -> list AxiomatizedTypes.Type_ -> Core.TyCon -> Core.DataCon.
+
+Axiom pcDataCon : Name.Name ->
+                  list Core.TyVar -> list AxiomatizedTypes.Type_ -> Core.TyCon -> Core.DataCon.
+
+Axiom parrTyCon_RDR : PrelNames.RdrName.
+
+Axiom parrTyConName : Name.Name.
+
+Axiom parrTyCon : Core.TyCon.
+
+Axiom parrFakeCon : BasicTypes.Arity -> Core.DataCon.
+
+Axiom parrDataConName : Name.Name.
+
+Axiom parrDataCon : Core.DataCon.
+
+Axiom pairTyCon : Core.TyCon.
+
+Axiom orderingTyCon : Core.TyCon.
+
+Axiom nothingDataConName : Name.Name.
+
+Axiom nothingDataCon : Core.DataCon.
+
+Axiom nilDataConName : Name.Name.
+
+Axiom nilDataCon : Core.DataCon.
+
+Axiom mk_tuple : BasicTypes.Boxity -> nat -> (Core.TyCon * Core.DataCon)%type.
+
+Axiom mk_special_dc_name : FastString.FastString ->
+                           Unique.Unique -> Core.DataCon -> Name.Name.
+
+Axiom mk_class : Core.TyCon ->
+                 AxiomatizedTypes.PredType -> Core.Id -> Core.Class.
+
+Axiom mkWiredInTyConName : Name.BuiltInSyntax ->
+                           Module.Module ->
+                           FastString.FastString -> Unique.Unique -> Core.TyCon -> Name.Name.
+
+Axiom mkWiredInIdName : Module.Module ->
+                        FastString.FastString -> Unique.Unique -> Core.Id -> Name.Name.
+
+Axiom mkWiredInDataConName : Name.BuiltInSyntax ->
+                             Module.Module ->
+                             FastString.FastString -> Unique.Unique -> Core.DataCon -> Name.Name.
+
+Axiom mkUnboxedTupleStr : BasicTypes.Arity -> GHC.Base.String.
+
+Axiom mkTupleTy : BasicTypes.Boxity ->
+                  list AxiomatizedTypes.Type_ -> AxiomatizedTypes.Type_.
+
+Axiom mkTupleOcc : OccName.NameSpace ->
+                   BasicTypes.Boxity -> BasicTypes.Arity -> OccName.OccName.
+
+Axiom mkSumTyConOcc : BasicTypes.Arity -> OccName.OccName.
+
+Axiom mkSumTy : list AxiomatizedTypes.Type_ -> AxiomatizedTypes.Type_.
+
+Axiom mkSumDataConOcc : BasicTypes.ConTag ->
+                        BasicTypes.Arity -> OccName.OccName.
+
+Axiom mkPromotedListTy : AxiomatizedTypes.Kind ->
+                         list AxiomatizedTypes.Type_ -> AxiomatizedTypes.Type_.
+
+Axiom mkPArrTy : AxiomatizedTypes.Type_ -> AxiomatizedTypes.Type_.
+
+Axiom mkPArrFakeCon : nat -> Core.DataCon.
+
+Axiom mkListTy : AxiomatizedTypes.Type_ -> AxiomatizedTypes.Type_.
+
+Axiom mkFunKind : AxiomatizedTypes.Kind ->
+                  AxiomatizedTypes.Kind -> AxiomatizedTypes.Kind.
+
+Axiom mkForAllKind : Core.TyVar ->
+                     Core.ArgFlag -> AxiomatizedTypes.Kind -> AxiomatizedTypes.Kind.
+
+Axiom mkDataConWorkerName : Core.DataCon -> Unique.Unique -> Name.Name.
+
+Axiom mkConstraintTupleStr : BasicTypes.Arity -> GHC.Base.String.
+
+Axiom mkCTupleOcc : OccName.NameSpace -> BasicTypes.Arity -> OccName.OccName.
+
+Axiom mkBoxedTupleTy : list AxiomatizedTypes.Type_ -> AxiomatizedTypes.Type_.
+
+Axiom mkBoxedTupleStr : BasicTypes.Arity -> GHC.Base.String.
+
+Axiom maybeTyConName : Name.Name.
+
+Axiom maybeTyCon : Core.TyCon.
+
+Axiom ltDataConId : Core.Id.
+
+Axiom ltDataCon : Core.DataCon.
+
+Axiom listTyCon_RDR : PrelNames.RdrName.
+
+Axiom listTyConName : Name.Name.
+
+Axiom listTyCon : Core.TyCon.
+
+Axiom liftedTypeKindTyConName : Name.Name.
+
+Axiom liftedTypeKindTyCon : Core.TyCon.
+
+Axiom liftedRepTy : AxiomatizedTypes.Type_.
+
+Axiom liftedRepDataConTyCon : Core.TyCon.
+
+Axiom justDataConName : Name.Name.
+
+Axiom justDataCon : Core.DataCon.
+
+Axiom isPArrTyCon : Core.TyCon -> bool.
+
+Axiom isPArrFakeCon : Core.DataCon -> bool.
+
+Axiom isCTupleTyConName : Name.Name -> bool.
+
+Axiom isBuiltInOcc_maybe : OccName.OccName -> option Name.Name.
+
+Axiom intTyCon_RDR : PrelNames.RdrName.
+
+Axiom intTyConName : Name.Name.
+
+Axiom intTyCon : Core.TyCon.
+
+Axiom intTy : AxiomatizedTypes.Type_.
+
+Axiom intDataCon_RDR : PrelNames.RdrName.
+
+Axiom intDataConName : Name.Name.
+
+Axiom intDataCon : Core.DataCon.
+
+Axiom heqTyConName : Name.Name.
+
+Axiom heqSCSelIdName : Name.Name.
+
+Axiom heqDataConName : Name.Name.
+
+Axiom gtDataConId : Core.Id.
+
+Axiom gtDataCon : Core.DataCon.
+
+Axiom floatTyConName : Name.Name.
+
+Axiom floatTyCon : Core.TyCon.
+
+Axiom floatTy : AxiomatizedTypes.Type_.
+
+Axiom floatDataConName : Name.Name.
+
+Axiom floatDataCon : Core.DataCon.
+
+Axiom false_RDR : PrelNames.RdrName.
+
+Axiom falseDataConName : Name.Name.
+
+Axiom falseDataConId : Core.Id.
+
+Axiom falseDataCon : Core.DataCon.
+
+Axiom extractPromotedList : AxiomatizedTypes.Type_ ->
+                            list AxiomatizedTypes.Type_.
+
+Axiom eqDataConId : Core.Id.
+
+Axiom eqDataCon : Core.DataCon.
+
+Axiom doubleTyConName : Name.Name.
+
+Axiom doubleTyCon : Core.TyCon.
+
+Axiom doubleTy : AxiomatizedTypes.Type_.
+
+Axiom doubleDataConName : Name.Name.
+
+Axiom doubleDataCon : Core.DataCon.
+
+Axiom constraintKindTyConName : Name.Name.
+
+Axiom constraintKindTyCon : Core.TyCon.
+
+Axiom consDataCon_RDR : PrelNames.RdrName.
+
+Axiom consDataConName : Name.Name.
+
+Axiom consDataCon : Core.DataCon.
+
+Axiom commas : BasicTypes.Arity -> GHC.Base.String.
+
+Axiom coercibleTyConName : Name.Name.
+
+Axiom coercibleSCSelIdName : Name.Name.
+
+Axiom coercibleDataConName : Name.Name.
+
+Axiom charTyCon_RDR : PrelNames.RdrName.
+
+Axiom charTyConName : Name.Name.
+
+Axiom charTyCon : Core.TyCon.
+
+Axiom charTy : AxiomatizedTypes.Type_.
+
+Axiom charDataConName : Name.Name.
+
+Axiom charDataCon : Core.DataCon.
+
+Axiom cTupleTyConNames : list Name.Name.
+
+Axiom cTupleTyConNameSet : NameSet.NameSet.
+
+Axiom cTupleTyConName : BasicTypes.Arity -> Name.Name.
+
+Axiom cTupleDataConNames : list Name.Name.
+
+Axiom cTupleDataConName : BasicTypes.Arity -> Name.Name.
+
+Axiom boxing_constr_env : NameEnv.NameEnv Core.DataCon.
+
+Axiom boxingDataCon_maybe : Core.TyCon -> option Core.DataCon.
+
+Axiom boolTyCon_RDR : PrelNames.RdrName.
+
+Axiom boolTyConName : Name.Name.
+
+Axiom boolTyCon : Core.TyCon.
+
+Axiom boolTy : AxiomatizedTypes.Type_.
+
+Axiom anyTypeOfKind : AxiomatizedTypes.Kind -> AxiomatizedTypes.Type_.
+
+Axiom anyTyConName : Name.Name.
+
+Axiom anyTyCon : Core.TyCon.
+
+Axiom anyTy : AxiomatizedTypes.Type_.
+
+Axiom alpha_tyvar : list Core.TyVar.
+
+Axiom alpha_ty : list AxiomatizedTypes.Type_.
+
+(* External variables:
+     bool list nat op_zt__ option AxiomatizedTypes.CType AxiomatizedTypes.Kind
+     AxiomatizedTypes.PredType AxiomatizedTypes.Type_ BasicTypes.Arity
+     BasicTypes.Boxity BasicTypes.ConTag BasicTypes.TupleSort Core.ArgFlag Core.Class
+     Core.DataCon Core.Id Core.RuntimeRepInfo Core.TyCon Core.TyVar
+     FastString.FastString GHC.Base.String Module.Module Name.BuiltInSyntax Name.Name
+     NameEnv.NameEnv NameSet.NameSet OccName.NameSpace OccName.OccName
+     PrelNames.RdrName Unique.Unique
+*)
